LeanMathLogicExploration/RelationalAlgebra2.lean
@@ -1,0 +1,65 @@
+import Mathlib.Tactic
+set_option pp.coercions false
+
+universe u v
+
+abbrev Relation.Pairs {α β: Type u} : Type u  :=  (a:α) -> (b:β) -> Prop
+
+abbrev Context := List String
+def addContexts := fun (a b: Context) => (List.append a b).dedup
+
+-- Not sure how this is supposed to work.
+
+-- The Relation inductive type gives the syntactic composition structure of relations. Relation.eval defines the semantic domain for this syntax.
+inductive Relation  : (contex: List String)-> (Dom:Type u) -> (Cod:Type u) -> Type (u+1)
+-- atomic forms a relation directly from a set of pairs
+| atomic (f:  α -> β -> Prop) : Relation [] α β
+
+-- TODO: We need to ensure the varName has the correct type.
+| vari  {α β: Type u}(varName: String)  : Relation [varName] α β
+
+-- pair forms a relation as a pair of two values. This is useful for forming higher-order relations from existing relations.
+| pair {α β: Type u} (a: α)(b: β): Relation [] α β
+
+-- comp stands for composition, and it is the sequential composition operation, which is defined analogously to function composition.
+| comp {α β γ : Type u} (R:Relation ctx1 α β) (S:Relation ctx2 β γ) : Relation (addContexts ctx1 ctx2) α γ
+
+-- converse is one of the involutions of relations, it reverses the direction of the pairs.
+| converse {α β : Type u} (R:Relation ctx α β) : Relation ctx β α
+
+-- complement is the other involution, it consists of the set theoretic complement of pairs relative to a given relation.
+| complement {α β : Type u} (R:Relation ctx α β) : Relation ctx α β
+
+-- full is the relation which is the full subset of the Cartersian product of domain and codomain. It's complement is an empty relation.
+| full (α β: Type u): Relation [] α β
+
+-- product is a monoidal product in the category Rel. It corresponds to one of the conjunction operations in linear logic, usually represented as ⊗.
+| product  {α β γ δ : Type u} (R: Relation ctx1 α β )(S: Relation ctx2 γ δ) : Relation (addContexts ctx1 ctx2) (α × γ) (β × δ)
+
+-- This is the coproduct in the category Rel. It corresponds to one of the disjunction operations in linear logic, usually represented as ⊕. It is interpreted as a disjoint union of domain, codomain, and relational pairs.
+| coproduct {α β γ δ : Type u} (R: Relation ctx1 α β )(S: Relation ctx2 γ δ) : Relation  (addContexts ctx1 ctx2) (Sum α γ ) (Sum β δ)
+
+-- Copy is the diagonal relation, connecting each value in the domain to a pair of identical copies in the codomain. The converse of this is a "merge" relation that sents pairs of identicals to a single copy.  The converse complement (linear negation) of copy is a "different" relation that sends pairs of different elements to all elements.
+| copy (α : Type u): Relation [] α (α × α)
+
+-- cocopy is the categorical dual of copy.  It relates the left and right values of a reflexitve sum type to their common value. This allows us to collapse or merge the disjoint sets of the Sum into a single set which is used to define union. The converse is a "split" relation that splits a single value into two parallel copies in disjoint sets.
+| cocopy (α: Type u): Relation [] (Sum α α) α
+
+-- First is a projection relation from a pair in the domain to the first member of the pair. The converse inserts a value into all pairs where it occurs in first position.
+| first (α β: Type u): Relation [] (α × β) α
+
+-- Second is a projection relation from a pair in the domain to the second member of the pair. The converse inserts a value into all pairs where it occurs in second position.
+| second (α β: Type u): Relation [] (α × β) β
+
+-- Left is an injection relation from a value to itself in the left side of a sum type. The converse is a kind of first projection that works with Sum types.
+| left (α β :Type u): Relation [] α (Sum α β)
+
+-- Right is an injection relation from a value to itself in the right side of a sum type. The converse is a kind of second projection that works with Sum types.
+| right (α β :Type u): Relation [] α (Sum β α)
+
+open Relation
+
+
+def Interpret (R: Relation ctx α β) (varName: String) :=
+  if not (ctx.contains varName) then R else
+  (f: α -> β -> Prop) :=
