LeanMathLogicExploration/RelationalAlgrebra3.lean
@@ -1,0 +1,17 @@
+
+
+-- Goal write version of relation exp that has arity rather than types.
+
+-- Define a Relation as an interpretation of a relation exp that assigns every atomic relation a function that is compatible with the arity, and where the types match for things like composition, ⊕, ⊗, etc.
+
+-- The context holds the names of atomic relations and a list of constraints on them, e.g., equality to other types, etc.
+
+
+-- Then eval works on the Relation
+
+
+def getArityType (α :Type u)(arity: Nat): Type u :=
+
+match arity with
+  | n+1 => α × (getArityType α  n)
+  | _ => α
