LeanMathLogicExploration/RelationalConstraintsExample.lean
@@ -1,0 +1,31 @@
+import  «LeanMathLogicExploration».RelationalAlgebra
+
+open Relation
+
+inductive Province :=
+| Alta
+| BC
+| Sask
+| On
+| Qc
+
+open Province
+
+def adjacent : (Pairs Province Province) := fun (a b) => match a, b with
+  | Alta, BC => True
+  | BC, Alta => True
+  | Alta, Sask => True
+  | Sask, Alta => True
+  | On, Qc => True
+  | Qc, On => True
+  | _, _ => False
+
+
+inductive Colour :=
+| red
+| green
+| blue
+
+open Colour
+
+-- Now I'd like to be able to define an expression without defining the actual relation for Dif.
