LeanMathLogicExploration/Tarski1941.lean
@@ -1,0 +1,24 @@
+import  «LeanMathLogicExploration».RelationalAlgebra
+
+-- Tarskis Notation
+abbrev one (α) := full α α
+abbrev zero (α) := Relation.empty α α
+abbrev one' (α) := Relation.id α
+abbrev zero' (α) := Relation.notEqual α
+
+
+
+-- *** Prove Tarski Axioms as Special Cases ***
+theorem tarski1941_axiom_1 : ∀ (x y: α), (Relation.eval (one α)) x y := by
+simp [Relation.eval]
+
+theorem tarski1941_axiom_2 : ∀ (x y: α), ¬(Relation.eval (zero α)) x y := by
+simp [Relation.eval]
+
+theorem tarski1941_axiom_3 : ∀ (x: α), (Relation.eval (one' α)) x x := by
+simp [Relation.eval] ; intro x ; exact ⟨(x, x), by simp⟩
+
+theorem tarski1941_axiom_4 : ∀ (x y z: α),∀ (R: EndoRel α), (eval R x y ∧ eval (one' α) y z) → (eval R x z) := by
+intros x y z R; unfold one' Relation.id; simp [Relation.eval, Relation.merge, Relation.domain]; intro evalR yEqz ; rw [yEqz.symm]; use evalR
+
+-- TODO: Prove the remaining axioms and theorems about union and intersection presented in Tarski 1941 paper.
