lakefile.lean
@@ -5,7 +5,7 @@ package «lean-math-logic-exploration» where
   -- Settings applied to both builds and interactive editing
   leanOptions := #[
     ⟨`pp.unicode.fun, true⟩, -- pretty-prints `fun a ↦ b`
-    ⟨`pp.proofs.withType, false⟩
+    ⟨`pp.proofs.withType, true⟩ -- I changed this to true to see what would happen
   ]
   -- add any additional package configuration options here
 
